

$$\text{Solving } \begin{cases} a_{n+1} = 2a_n + n \dots \dots \dots (1.2.1) \\ a_0 = 1 \end{cases}$$

ANS:

$$\Rightarrow A(X) = \sum_{n=0}^{\infty} a_n x^n = a_0 + a_1 x + a_2 x^2 + a_3 x^3 \dots$$

Multiply x^n on (1.2.1)

$$a_{n+1} x^n = 2 \times a_n x^n + n x^n$$

Adding Sigma on the formula above

$$\sum_{n=0}^{\infty} a_{n+1} x^n = \sum_{n=0}^{\infty} 2 \times a_n x^n + \sum_{n=0}^{\infty} n x^n \dots \dots (*)$$

Considering $\frac{A(x)}{x} = \frac{a_0}{x} + a_1 + a_2 x^1 + a_3 x^2 \dots$, and $a_0 = 1$ 代入

$$\therefore \text{LHS of } (*) = \sum_{n=0}^{\infty} a_{n+1} x^n = \frac{A(x) - 1}{x}$$

$$\text{RHS of } (*) = 2 \times \sum_{n=0}^{\infty} a_n x^n + \sum_{n=0}^{\infty} n x^n$$

$$\text{considering } \sum_{n=0}^{\infty} n x^n = \sum_{n=0}^{\infty} x \times \left(\frac{d}{dx}\right) x^n = x \times \frac{d}{dx} \sum_{n=0}^{\infty} x^n = x \times \frac{d}{dx} \left(\frac{1}{1-x}\right) = \frac{x}{(1-x)^2}$$

$$\therefore \frac{A(x) - 1}{x} = 2A(x) + \frac{x}{(1-x)^2}$$

移項可得 $A(x) = \frac{1-2x+2x^2}{(1-2x)(1-x)^2} := \frac{A}{(1-x)^2} + \frac{B}{1-x} + \frac{C}{1-2x}$; 要解 A,B,C 皆常數

解得 $A=(-1), B=0, C=2$

$$\therefore A(x) = \sum_{n=0}^{\infty} a_n x^n = \frac{-1}{(1-x)^2} + \frac{2}{1-2x} = 2 \times \sum_{n=0}^{\infty} (2x)^n - \sum_{n=0}^{\infty} n x^n = \sum_{n=0}^{\infty} (2 \times 2^n - n) x^n$$

我能從紅色的地方推論 $a_n = (2 \times 2^n - n)$ 嗎

但是看答案是 $a_n = (2 \times 2^n - n - 1)$;

能幫我糾錯嗎?